driver/IdSimClightExtra.v
@@ -1,0 +1,112 @@
+Require Import Program.
+
+Require Import Sem SimProg Skeleton Mod ModSem SimMod SimModSem SimSymb SimMem Sound SimSymb.
+Require Import Cop Ctypes ClightC.
+Require Import AsmC.
+Require SimMemInjInvC.
+Require Import CoqlibC.
+Require Import ValuesC.
+Require Import LinkingC.
+Require Import MapsC.
+Require Import AxiomsC.
+Require Import Ord.
+Require Import MemoryC.
+Require Import SmallstepC.
+Require Import Events.
+Require Import Preservation.
+Require Import Integers.
+Require Import LocationsC Conventions.
+Require Import Conventions1C.
+
+Require Import AsmregsC.
+Require Import MatchSimModSem.
+Require Import StoreArguments.
+Require Import AsmStepInj IntegersC.
+Require Import Coq.Logic.PropExtensionality.
+Require Import AsmExtra IdSimExtra IdSimAsmExtra IdSimInvExtra.
+
+Require Import MatchSimModSem.
+Require Import Conventions1C.
+
+Require Import ClightStepInj.
+Require Import IdSimExtra IdSimInvExtra.
+Require Import mktac.
+
+Set Implicit Arguments.
+
+Local Opaque Z.mul Z.add Z.sub Z.div.
+
+Lemma val_casted_inject val0 val1 j ty
+      (VAL: Val.inject j val0 val1)
+      (CAST: val_casted val0 ty)
+  :
+    val_casted val1 ty.
+Proof.
+  inv CAST; inv VAL; clarify; try econs; eauto.
+Qed.
+
+Require Import CtypingC.
+Require Import CopC.
+
+Lemma typecheck_inject vals0 vals1 j ty
+      (VALS: Val.inject_list j vals0 vals1)
+      (TYP: typecheck vals0 ty)
+  :
+    typecheck vals1 ty.
+Proof.
+  inv TYP. econs; eauto. clear - VALS TYP0.
+  revert vals1 VALS TYP0. generalize (typelist_to_listtype ty).
+  clear ty. induction vals0; ss.
+  - i. inv VALS. inv TYP0. econs.
+  - i. inv VALS. inv TYP0. econs.
+    + eapply val_casted_inject; eauto.
+    + eapply IHvals0; eauto.
+Qed.
+
+Lemma wt_retval_inject j v_src v_tgt ty
+      (INJ: Val.inject j v_src v_tgt)
+      (TYP: wt_retval v_tgt ty)
+  :
+    wt_retval v_src ty.
+Proof.
+  inv TYP; inv WTV; inv INJ; clarify; try by repeat (econs; eauto).
+  exploit NVOID; eauto. clarify.
+Qed.
+
+Lemma typify_c_inject j retv_src retv_tgt tres tv_src
+      (TYP: typify_c retv_src tres tv_src)
+      (INJ: Val.inject j retv_src retv_tgt)
+  :
+    exists tv_tgt,
+      (<<TYP: typify_c retv_tgt tres tv_tgt>>) /\
+      (<<INJ: Val.inject j tv_src tv_tgt>>).
+Proof.
+  inv TYP.
+  - destruct (classic (wt_retval retv_tgt tres)).
+    + esplits; eauto. econs; eauto.
+    + exists Vundef. esplits; eauto.
+      * econs 2. eauto.
+      * assert (tv_src = Vundef); clarify; eauto.
+        inv INJ; inv WT; inv WTV; clarify;
+          exfalso; eapply H; econs; clarify; try (econs; eauto).
+        exploit NVOID; eauto. clarify.
+  - exists Vundef. esplits; eauto.
+    econs 2. ii. exploit wt_retval_inject; eauto.
+Qed.
+
+Lemma vals_casted_inject j vals_src vals_tgt tys
+      (VALS: Val.inject_list j vals_src vals_tgt)
+      (TYP: Forall2 val_casted vals_src tys)
+  :
+    Forall2 val_casted vals_tgt tys.
+Proof.
+  ginduction vals_src; i.
+  - inv VALS. inv TYP. econs.
+  - inv VALS. inv TYP. econs; eauto.
+    eapply val_casted_inject; eauto.
+Qed.
+
+Definition cgenv skenv_link clight :=
+  Build_genv
+    (SkEnv.revive (SkEnv.project skenv_link (CtypesC.CSk.of_program signature_of_function clight)) clight)
+    (prog_comp_env clight).
